pulse/Pulse.Lib.C.Array.fst
@@ -27,7 +27,8 @@ let array_spec_initd #a (s: array_spec a) (i: nat) : prop = i < Seq.length s /\ 
 let array_spec_mask #a (s: array_spec a) (i: nat) : prop = i < Seq.length s /\ ~(OutOfMask? (Seq.index s i))
 let array_spec_idx #a (s: array_spec a) (i: nat { array_spec_initd s i }) : Tot a = let Val x = Seq.index s i in x
 
-let array_literal_to_ref #a #n (_: full_array_lspec a n) : Tot (R.ref a) =
+let string_literal_to_ref #a (_literal_identity: string) :
+  Tot (r:R.ref a { not (r == R.null) }) =
   admit ()
 
 let to_mask #t (s: array_spec t) (i: nat) : prop = array_spec_mask s i
